psi example

examples/wysteria/ml/runtime.ml
@@ -14,7 +14,10 @@ let open_connection (port:int) :(chan_in * chan_out) =
   Unix.open_connection sock_addr
 
 let client_write (out:chan_out) (p:prin) (r:redex) :unit = Marshal.output ~closures:true out (p, r); IO.flush out
-let client_read (c_in:chan_in) :dvalue = Marshal.input c_in
+let client_read (c_in:chan_in) :dvalue =
+  let v = Marshal.input c_in in
+  IO.close_in c_in;
+  v
 
 let establish_server (callback:chan_in -> chan_out -> unit) (port:int) =
   let sock = Unix.socket Unix.PF_INET Unix.SOCK_STREAM 0 in
@@ -30,7 +33,7 @@ let establish_server (callback:chan_in -> chan_out -> unit) (port:int) =
   accept_loop ()  
 
 let server_read (c:chan_in) :(prin * redex) = Marshal.input c
-let server_write (out:chan_out) (dv:dvalue) :unit = Marshal.output ~closures:true out dv; IO.flush out
+let server_write (out:chan_out) (dv:dvalue) :unit = Marshal.output ~closures:true out dv; IO.flush out; IO.close_out out
 let create_thread (f:unit -> unit) :unit = let _ = Thread.create f () in ()
 
 let is_server _ = Sys.argv.(1) = "0"
