examples/wysteria/examples/lib.fst
@@ -1,6 +1,6 @@
 (*--build-config
     options:--admit_fsi FStar.Set --admit_fsi Wysteria --admit_fsi Prins --admit_fsi FStar.OrdSet --admit_fsi FStar.IO;
-    other-files:ghost.fst ext.fst set.fsi heap.fst st.fst all.fst io.fsti list.fst st2.fst ordset.fsi ../prins.fsi ffi.fst wysteria.fsi
+    other-files:ghost.fst ext.fst set.fsi heap.fst st.fst all.fst io.fsti list.fst listTot.fst st2.fst ordset.fsi ../prins.fsi ffi.fst wysteria.fsi
  --*)
 
 module WLib
