examples/wysteria/examples/psi.fst
@@ -1,0 +1,95 @@
+(*--build-config
+    options:--admit_fsi FStar.Set --admit_fsi Wysteria --admit_fsi Prins --admit_fsi FStar.OrdSet --admit_fsi FStar.IO;
+    other-files:ghost.fst ext.fst set.fsi heap.fst st.fst all.fst io.fsti list.fst listTot.fst st2.fst ordset.fsi ../prins.fsi ffi.fst wysteria.fsi
+ --*)
+
+(* PSI *)
+
+module SMC
+
+open FStar.List.Tot
+open Prins
+open FFI
+open Wysteria
+
+let alice_s = singleton alice
+let bob_s = singleton bob
+let ab = union alice_s bob_s
+
+type pre  (m:mode)  = fun m0 -> b2t (m0 = m)
+type post (#a:Type) = fun (m:mode) (x:a) (t:trace) -> True
+
+type pre_with (m:mode) (t:Type) = fun m0 -> m0 = m /\ t
+
+let to_s2 p1 p2 = union (singleton p1) (singleton p2)
+
+val read_fn: p:prin -> unit -> Wys (list int) (fun m0 -> b2t (m0 = Mode Par (singleton p)))
+                                          (fun m0 r t -> True)
+let read_fn _ _ = w_read_int_list ()
+
+val nth: n:nat -> l:list int{length l >= n + 1} -> Tot int
+let rec nth n l = if n = 0 then hd_of_cons l else nth (n - 1) (tl_of_cons l)
+
+val mem: x:Box int alice_s -> l:Box (list int) bob_s
+         -> n:nat{length (v_of_box l) >= n}
+	 -> Wys (bool * int) (pre (Mode Par ab)) post
+let rec mem x l n =
+  if n = 0 then mk_tuple false 0
+  else
+    let g:unit -> Wys int (pre (Mode Par bob_s)) post =
+      fun _ -> nth (n - 1) (unbox_p l)
+    in
+    let y = as_par bob_s g in
+    let cmp:unit -> Wys (bool * int) (pre (Mode Sec ab)) post =
+      fun _ -> if unbox_s x = unbox_s y then mk_tuple true (unbox_s x) else mk_tuple false 0
+    in
+    let p = as_sec ab cmp in
+    if fst p then p else mem x l (n - 1)
+
+val psi: l1:Box (list int) alice_s -> l2:Box (list int) bob_s
+         -> n1:nat{length (v_of_box l1) >= n1} -> n2:nat{length (v_of_box l2) >= n2}
+	 -> acc:list int
+	 -> Wys (list int) (pre (Mode Par ab)) post
+let rec psi l1 l2 n1 n2 acc =
+  if n1 = 0 then acc
+  else
+    let g:unit -> Wys int (pre (Mode Par alice_s)) post =
+      fun _ -> nth (n1 - 1) (unbox_p l1)
+    in
+    let x = as_par alice_s g in
+    let p = mem x l2 n2 in
+    let acc' = if fst p then mk_cons (snd p) acc else acc in
+    psi l1 l2 (n1 - 1) n2 acc'
+
+val mlength: l:list int -> Tot (n:nat{n = length l})
+let rec mlength l = if is_Nil l then 0 else 1 + mlength (tl_of_cons l)
+
+val psi_m: unit -> Wys (list int) (pre (Mode Par ab)) post
+let psi_m _ =
+  let l1 = as_par alice_s (read_fn alice) in
+  let l2 = as_par bob_s (read_fn bob) in
+
+  let len: p:prin -> l:(Box (list int) (singleton p))
+           -> unit
+	   -> Wys nat (pre (Mode Par (singleton p))) (fun _ r _ -> True /\ r = length (v_of_box l)) =
+    fun _ l _ ->
+    let l = unbox_p l in
+    mlength l
+  in
+  let n1 = as_par alice_s (len alice l1) in
+  let n2 = as_par bob_s (len bob l2) in
+
+  let g: p:prin{p = alice \/ p = bob} -> n:Box int (singleton p)
+         -> unit
+	 -> Wys int (pre (Mode Sec ab)) (fun _ r _ -> True /\ r = v_of_box n) =
+    fun p n _ -> unbox_s n
+  in
+
+  let n1' = as_sec ab (g alice n1) in
+  let n2' = as_sec ab (g bob n2) in
+
+  psi l1 l2 n1' n2' (mk_nil ())
+;;
+
+let l = main ab psi_m in
+print_int_list l
